@prefix : <http://rdf.jpostdb.org/ontology/mbpost-cv.ttl#> .
@prefix dct: <http://purl.org/dc/terms/> .
@prefix owl: <http://www.w3.org/2002/07/owl#> .
@prefix rdf: <http://www.w3.org/1999/02/22-rdf-syntax-ns#> .
@prefix rdfs: <http://www.w3.org/2000/01/rdf-schema#> .

<http://rdf.jpostdb.org/ontology/mbpost-cv.ttl> rdf:type owl:Ontology ;
                                             dct:creator "Akiyasu C. Yoshizawa" ;
                                             dct:creator "Yushi Takahashi" ;
                                             dct:description "The controlled vocabulary for managing MB-POST, a repository of metabolome datasets." ;
                                             dct:license <http://creativecommons.org/publicdomain/zero/1.0/> ;
                                             rdfs:label "MB-POST controlled vocabulary" ;
                                             owl:versionInfo 1.0 .

#################################################################
#    Classes
#################################################################

###  http://rdf.jpostdb.org/ontology/mbpost-cv.ttl#MBP_001
:MBP_001 rdf:type owl:Class ;
         dct:identifier "MBP_001" ;
         rdfs:label "MB-POST controlled vocabulary" ;
         dct:description "The root node for terms relating to the description of MB-POST." .

###  http://rdf.jpostdb.org/ontology/mbpost-cv.ttl#MBP_002
:MBP_002 rdf:type owl:Class ;
         dct:identifier "MBP_002" ;
         rdfs:label "Metabolome and Lipidome" ;
         dct:description "The complete set of hydrophilic metabolites and lipids produced under a given specific conditions." ;
         rdfs:subClassOf :MBP_001 .

###  http://rdf.jpostdb.org/ontology/mbpost-cv.ttl#MBP_003
:MBP_003 rdf:type owl:Class ;
         dct:identifier "MBP_003" ;
         rdfs:label "Volatilome" ;
         dct:description "The complete set of volatile organic and inorganic compounds that originate from an organism, super-organism, or ecosystem under specific conditions." ;
         rdfs:subClassOf :MBP_001 .

###  http://rdf.jpostdb.org/ontology/mbpost-cv.ttl#MBP_004
:MBP_004 rdf:type owl:Class ;
         dct:identifier "MBP_004" ;
         rdfs:label "Metallome" ;
         dct:description "The complete set of metal and metalloid species within a cell or tissue type under specific conditions." ;
         rdfs:subClassOf :MBP_001 .

###  http://rdf.jpostdb.org/ontology/mbpost-cv.ttl#MBP_005
:MBP_005 rdf:type owl:Class ;
         dct:identifier "MBP_005" ;
         rdfs:label "IC-MS" ;
         dct:description "A separation and detection method that combines ion chromatography and mass spectrometry." ;
         rdfs:subClassOf :MBP_001 .

###  http://rdf.jpostdb.org/ontology/mbpost-cv.ttl#MBP_006
:MBP_006 rdf:type owl:Class ;
         dct:identifier "MBP_006" ;
         rdfs:label "SFC-MS" ;
         dct:description "A separation and detection method that combines supercritical fluid chromatography and mass spectrometry." ;
         rdfs:subClassOf :MBP_001 .

###  http://rdf.jpostdb.org/ontology/mbpost-cv.ttl#MBP_007
:MBP_007 rdf:type owl:Class ;
         dct:identifier "MBP_007" ;
         rdfs:label "SFC_Reversed phase" ;
         dct:description "Supercritical fluid chromatography using a reversed-phase column." ;
         rdfs:subClassOf :MBP_001 .

###  http://rdf.jpostdb.org/ontology/mbpost-cv.ttl#MBP_008
:MBP_008 rdf:type owl:Class ;
         dct:identifier "MBP_008" ;
         rdfs:label "SFC_Normal phase" ;
         dct:description "Supercritical fluid chromatography using a normal-phase column." ;
         rdfs:subClassOf :MBP_001 .

###  http://rdf.jpostdb.org/ontology/mbpost-cv.ttl#MBP_009
:MBP_009 rdf:type owl:Class ;
         dct:identifier "MBP_009" ;
         rdfs:label "Positive and Negative" ;
         dct:description "A data acquisition mode that alternates between positive and negative ion mode." ;
         rdfs:subClassOf :MBP_001 .

###  http://rdf.jpostdb.org/ontology/mbpost-cv.ttl#MBP_010
:MBP_010 rdf:type owl:Class ;
         dct:identifier "MBP_010" ;
         rdfs:label "OAD" ;
         dct:description "Oxygen Attachment Dissociation; a fragmentation method using atomic oxygen (O) and/or hydroxyl radical (OHÂ·)." ;
         rdfs:subClassOf :MBP_001 .

